Predicate abstraction fixed, FibFibFast works, clean up to be done.

Benchmarks/FluxRS/FibFibFast.lean
@@ -7,14 +7,10 @@ def fib_spec_fib (n : Int) : Int :=
   else fib_spec_fib (n - 1) + fib_spec_fib (n - 2)
   termination_by n.toNat
 
-@[qualif] def q_le          (a b : Int) : Prop := a ≤ b
-@[qualif] def q_gt_one      (v : Int)   : Prop := v > 1
-@[qualif] def q_eq_fib      (v i : Int) : Prop := v = fib_spec_fib i
-@[qualif] def q_eq_fib_pred (v i : Int) : Prop := v = fib_spec_fib (i - 1)
 
-@[simp]
-def fib_fast_inv (i : Int) (prev : Int) (curr : Int) (n : Int) : Prop :=
-  i > 1 ∧ i ≤ n ∧ prev = fib_spec_fib (i - 1) ∧ curr = fib_spec_fib i
+-- @[simp]
+-- def fib_fast_inv (i : Int) (prev : Int) (curr : Int) (n : Int) : Prop :=
+--   i > 1 ∧ i ≤ n ∧ prev = fib_spec_fib (i - 1) ∧ curr = fib_spec_fib i
 
 def FibFibFast := ∃ k0 : (a0 : Int) -> (a1 : Int) -> (a2 : Int) -> (a3 : Int) -> Prop,
  ∀ (n₀ : Int),
@@ -34,6 +30,10 @@ def FibFibFast := ∃ k0 : (a0 : Int) -> (a1 : Int) -> (a2 : Int) -> (a3 : Int) 
    ((n₀ ≤ 1) ->
     (1 = (fib_spec_fib n₀)))
 
-def FibFibFast_proof : FibFibFast := by
-  unfold FibFibFast; exists fib_fast_inv; simp
-  zap
+@[qualif] def q_le          (a b : Int) : Prop := a ≤ b
+@[qualif] def q_gt_one      (v : Int)   : Prop := v > 1
+@[qualif] def q_eq_fib      (v i : Int) : Prop := v = fib_spec_fib i
+@[qualif] def q_eq_fib_pred (v i : Int) : Prop := v = fib_spec_fib (i - 1)
+
+theorem FibFibFast_proof : FibFibFast := by
+  solve_fixpoint
