LeanFixpoint.lean
@@ -20,8 +20,7 @@ import LeanFixpoint.Elab.FromExpr
   verification conditions.
 -/
 import LeanFixpoint.Tactic.Command
--- import LeanFixpoint.Tactic.Grind        -- TODO: update for Expr passthrough
--- import LeanFixpoint.Tactic.SolveFixpoint -- TODO: update for Expr passthrough
+import LeanFixpoint.Tactic.SolveFixpoint
 import LeanFixpoint.Tactic.Tactics
 import LeanFixpoint.Tactic.Utils
 import LeanFixpoint.Tactic.SolveFusion
@@ -33,9 +32,9 @@ import LeanFixpoint.Tactic.SolveFusion
 -/
 import LeanFixpoint.Solve.Qualifier
 import LeanFixpoint.Solve.Instantiation
--- import LeanFixpoint.Solve.Solver
--- import LeanFixpoint.Solve.Weakening
--- import LeanFixpoint.Solve.Fixpoint
+import LeanFixpoint.Solve.Weaken
+import LeanFixpoint.Solve.Fixpoint
+
 
 /-
   Sound Verification Condition Generation
